dpe: DeriveChild checks on engine and l0 layers

share/steel/examples/pulse/dice/common/CommonTypes.fst
@@ -9,128 +9,20 @@ module L = Steel.ST.SpinLock
 module US = FStar.SizeT
 module U8 = FStar.UInt8
 module U32 = FStar.UInt32
-open HACL
-open EngineTypes
-open L0Types
-open Array 
 
-(* ----------- HELPERS ----------- *)
+assume 
+val u32_to_us (v:U32.t) : US.t
 
-```pulse
-fn zeroize_uds (uds:A.array U8.t) 
-               (l:(l:US.t{ US.v l = A.length uds })) 
-               (#uds0:(uds0:Ghost.erased (Seq.seq U8.t) { Seq.length uds0 = A.length uds }))
-  requires (
-    uds_is_enabled **
-    A.pts_to uds full_perm uds0
-  )
-  ensures (
-    uds_is_enabled **
-    exists (uds1:Seq.seq U8.t). (
-      A.pts_to uds full_perm uds1 **
-      pure (uds1 `Seq.equal` Seq.create (US.v l) 0uy))
-  )
-{
-  fill_array l uds 0uy;
-}
-```
-
-(* ----------- CONTEXT ----------- *)
-
-noeq
-type engine_context = { uds: A.larray U8.t (US.v uds_len); }
-let engine_context_perm (c:engine_context) : vprop
-  = A.pts_to c.uds full_perm uds_bytes `star` 
-    uds_is_enabled `star`
-    pure (A.is_full_array c.uds)
-let mk_engine_context uds : engine_context = {uds}
-
-noeq
-type l0_context = { cdi: A.array U8.t; }
-let l0_context_perm (c:l0_context) : vprop
-  = exists_ (fun s -> A.pts_to c.cdi full_perm s) `star`
-    pure (A.is_full_array c.cdi)
-let mk_l0_context cdi : l0_context = {cdi}
-
+// TODO: move elsewhere
 noeq
 type l1_context = { aliasKey_priv: A.larray U8.t 32;
-                    cert_aliasKey: A.array U8.t;
-                    csr_deviceID: A.array U8.t; }
+                    aliasKeyCRT: A.array U8.t;
+                    deviceIDCSR: A.array U8.t; }
+
 let l1_context_perm (c:l1_context)
   : vprop
   = exists_ (fun s -> A.pts_to c.aliasKey_priv full_perm s) `star`
-    exists_ (fun s -> A.pts_to c.cert_aliasKey full_perm s) `star`
-    exists_ (fun s -> A.pts_to c.csr_deviceID full_perm s)
-let mk_l1_context aliasKey_priv cert_aliasKey csr_deviceID = { aliasKey_priv; cert_aliasKey; csr_deviceID }
+    exists_ (fun s -> A.pts_to c.aliasKeyCRT full_perm s) `star`
+    exists_ (fun s -> A.pts_to c.deviceIDCSR full_perm s)
 
-noeq
-type context_t = 
-  | Engine_context : c:engine_context -> context_t
-  | L0_context     : c:l0_context -> context_t
-  | L1_context     : c:l1_context -> context_t
-
-let context_perm (t:context_t) : vprop = 
-  match t with
-  | Engine_context c -> engine_context_perm c
-  | L0_context c -> l0_context_perm c
-  | L1_context c -> l1_context_perm c
-
-let mk_engine_context_t engine_context = Engine_context engine_context
-let mk_l0_context_t l0_context = L0_context l0_context
-let mk_l1_context_t l1_context = L1_context l1_context
-
-let locked_context_t = c:context_t & L.lock (context_perm c)
-
-(* ----------- RECORD ----------- *)
-
-noeq
-type l0_record_t = {
-  cdi: A.larray U8.t 32;
-  fwid: A.larray U8.t 32;
-  deviceID_label_len: hkdf_lbl_len; (* should be U32 *)
-  deviceID_label: A.larray U8.t (US.v deviceID_label_len); (* public bytes *)
-  aliasKey_label_len: hkdf_lbl_len; (* should be U32 *)
-  aliasKey_label: A.larray U8.t (US.v aliasKey_label_len); (* public bytes *)
-  deviceIDCSR_ingredients: deviceIDCSR_ingredients_t;
-  aliasKeyCRT_ingredients: aliasKeyCRT_ingredients_t;
-}
-
-noeq
-type l0_record_repr = {
-  cdi: Seq.seq U8.t;
-  fwid: Seq.seq U8.t;
-  deviceID_label: Seq.seq U8.t;
-  aliasKey_label: Seq.seq U8.t;
-}
-
-let mk_l0_repr cdi fwid deviceID_label aliasKey_label 
-  = {cdi; fwid; deviceID_label; aliasKey_label}
-
-let l0_record_perm (record:l0_record_t) (repr:l0_record_repr) : vprop = 
-  A.pts_to record.cdi full_perm repr.cdi `star`
-  A.pts_to record.fwid full_perm repr.fwid `star`
-  A.pts_to record.deviceID_label full_perm repr.deviceID_label `star`
-  A.pts_to record.aliasKey_label full_perm repr.aliasKey_label
-
-noeq
-type record_t =
-  | Engine_record : r:engine_record_t -> record_t
-  | L0_record     : r:l0_record_t -> record_t
-
-noeq
-type repr_t = 
-  | Engine_repr : r:engine_record_repr -> repr_t
-  | L0_repr     : r:l0_record_repr -> repr_t
-
-let record_perm (t_rec:record_t) (t_rep:repr_t) : vprop = 
-  match t_rec with
-  | Engine_record r -> (
-    match t_rep with 
-    | Engine_repr r0 -> engine_record_perm r r0
-    | _ -> pure(false)
-  )
-  | L0_record r -> (
-    match t_rep with
-    | L0_repr r0 -> l0_record_perm r r0
-    | _ -> pure(false)
-  )
+let mk_l1_context aliasKey_priv aliasKeyCRT deviceIDCSR = { aliasKey_priv; aliasKeyCRT; deviceIDCSR }
